restored old types similar to Seq.* functions

proof-libs/fstar/core/Core.Ops.Range.fsti
@@ -51,30 +51,30 @@ instance impl_index_range_slice t n : t_Index (t_Slice t) (t_Range (int_t n))
     ; f_index_post = (fun _ _ _ -> true)
     ; f_index_pre = (fun (s: t_Slice t) {f_start; f_end} -> 
          let len = length s in
-         v f_start >= 0 /\ v f_start <= v len /\ v f_end <= v len)
+         v f_start >= 0 /\ v f_start <= len /\ v f_end <= len)
     ; f_index = (fun s (r: t_Range (int_t n)) -> 
           let {f_start; f_end} = r in
           if v f_start < v f_end 
-          then slice s (sz (v f_start)) (sz (v f_end))
+          then slice s (v f_start) (v f_end)
           else empty)}
 
 instance impl_index_range_to_slice t n : t_Index (t_Slice t) (t_RangeTo (int_t n)) 
   = { f_Output = t_Slice t
     ; f_index_post = (fun _ _ _ -> true)
     ; f_index_pre = (fun (s: t_Slice t) ({f_end}: t_RangeTo (int_t n)) -> 
-         let len = Rust_primitives.length s in v f_end <= v len)
+         let len = Rust_primitives.length s in v f_end <= len)
     ; f_index = (fun s (r:t_RangeTo (int_t n)) -> 
          let {f_end} = r in 
-         if 0 < v f_end then slice s (sz 0) (sz (v f_end)) else empty)}
+         if 0 < v f_end then slice s 0 (v f_end) else empty)}
 
 instance impl_index_range_from_slice t n : t_Index (t_Slice t) (t_RangeFrom (int_t n)) 
   = { f_Output = t_Slice t
     ; f_index_post = (fun _ _ _ -> true)
     ; f_index_pre = (fun (s: t_Slice t) ({f_start}: t_RangeFrom (int_t n)) -> 
-         let len = Rust_primitives.length s in v f_start >= 0 /\ v f_start <= v len)
+         let len = Rust_primitives.length s in v f_start >= 0 /\ v f_start <= len)
     ; f_index = (fun s {f_start} -> 
          let len = Rust_primitives.length s in
-         if v f_start = v len then empty else slice s (sz (v f_start)) len)}
+         if v f_start = len then empty else slice s (v f_start) len)}
          
 instance impl_index_range_full_slice t : t_Index (t_Slice t) t_RangeFull
   = { f_Output = t_Slice t
