proof-libs/fstar/core/Alloc.Vec.fst
@@ -5,7 +5,7 @@ unfold type t_Vec t (_: unit) = t_Slice t
 
 let impl__new #t (): t_Vec t () = empty
 
-let impl_2__extend_from_slice #t (#[(Tactics.exact (`()))]alloc:unit) (self: t_Vec t alloc) (other: t_Slice t{v (length self) + v (length other) <= max_usize}): t_Vec t alloc
+let impl_2__extend_from_slice #t (#[(Tactics.exact (`()))]alloc:unit) (self: t_Vec t alloc) (other: t_Slice t{length self + length other <= max_usize}): t_Vec t alloc
   = concat self other
 
 let impl__with_capacity (_capacity: usize) = impl__new ()
@@ -18,32 +18,32 @@ let impl_1__push #t
   (v: t_Vec t alloc)
   (x: t)
    : t_Vec t alloc = 
-     if length v = sz (max_usize) then v else
-     concat v (create (sz 1) x)
+     if length v = max_usize then v else
+     concat v (create 1 x)
 
 let impl_1__len #t (#[(Tactics.exact (`()))]alloc:unit) (v: t_Vec t alloc) =
-  length v
+  sz (length v)
 
 let impl_1__as_slice #t (#[(Tactics.exact (`()))]alloc:unit) (v: t_Vec t alloc) : t_Slice t = v
 
-let from_elem #a (item: a) (len: usize) = create len item
+let from_elem #a (item: a) (len: usize) = create (v len) item
 
 open Rust_primitives.Hax
 open Core.Ops.Index
 instance update_at_tc_array t n: update_at_tc (t_Vec t ()) (int_t n) = {
   super_index = FStar.Tactics.Typeclasses.solve <: t_Index (t_Vec t ()) (int_t n);
-  update_at = (fun arr i x -> upd arr (sz (v i)) x);
+  update_at = (fun arr i x -> upd arr (v i) x);
 }
 
 
 let impl_1__is_empty #t (#[(Tactics.exact (`()))]alloc:unit) (v: t_Vec t alloc): bool =
-  length v = sz 0
+  length v = 0
 
-let impl_1__insert #t (#[(Tactics.exact (`()))]alloc:unit) (v: t_Vec t alloc) 
-  (index: usize {index <=. length v /\ length v <. sz max_usize}) (element: t) 
+let impl_1__insert #t (#[(Tactics.exact (`()))]alloc:unit) (vec: t_Vec t alloc) 
+  (index: usize {v index <= length vec /\ length vec < max_usize}) (element: t) 
   : t_Vec t alloc =
-  let left = slice #t v (sz 0) index in 
-  let right = slice #t v index (length v) in 
+  let left = slice #t vec 0 (v index) in 
+  let right = slice #t vec (v index) (length vec) in 
   concat left (cons element right)
 
 assume val impl_1__drain #t (#[(Tactics.exact (`()))]alloc:unit) #range_t  (v: t_Vec t alloc) (r: range_t): 
@@ -53,13 +53,13 @@ assume val impl_1__truncate #t (#[(Tactics.exact (`()))]alloc:unit)  (v: t_Vec t
 
 assume val impl_1__swap_remove #t (#[(Tactics.exact (`()))]alloc:unit)  (v: t_Vec t alloc) (n: usize): t_Vec t alloc & t
 
-assume val impl_2__resize #t (#[(Tactics.exact (`()))]alloc:unit)  (v: t_Vec t alloc) (new_size: usize) (value: t): 
+assume val impl_2__resize #t (#[(Tactics.exact (`()))]alloc:unit)  (vec: t_Vec t alloc) (new_size: usize) (value: t): 
   Prims.Pure
       (t_Vec t alloc)
       Prims.l_True
       (ensures
         fun new_v ->
-          new_size ==
+          v new_size ==
           length new_v)
 
 assume val impl_1__remove #t (#[(Tactics.exact (`()))]alloc:unit)  (v: t_Vec t alloc) (index: usize): t_Vec t alloc & t
