proof-libs/fstar/core/Core.Slice.fsti
@@ -3,8 +3,8 @@ open Rust_primitives.Arrays
 open Rust_primitives.Integers
 
 let impl__len (#t: Type) (s: t_Slice t)
-  : len: usize {len == length s} = 
-  length s
+  : len: usize {v len == length s} = 
+  sz (length s)
 
 open Core.Slice.Iter
 
@@ -15,27 +15,27 @@ let impl__iter #t (s: t_Slice t): t_Slice t = s
 val impl__chunks_exact #a (x: t_Slice a) (cs: usize):
     Pure (t_Slice (t_Slice a))
     (requires True)
-    (ensures (fun r -> forall i. i < v (length x) ==> length x ==  cs))
+    (ensures (fun r -> forall i. i < length x ==> length x ==  v cs))
 
 open Core.Ops.Index
 
 instance impl__index t n: t_Index (t_Slice t) (int_t n)
   = { f_Output = t;
-      f_index_pre = (fun (s: t_Slice t) (i: int_t n) -> v i >= 0 && v i < v (length s));
+      f_index_pre = (fun (s: t_Slice t) (i: int_t n) -> v i >= 0 && v i < length s);
       f_index_post = (fun _ _ _ -> true);
-      f_index = (fun s i -> index s (sz (v i)));
+      f_index = (fun s i -> index s (v i));
     }
 
 let impl__copy_from_slice #t (x: t_Slice t) (y:t_Slice t) : t_Slice t = y
 let impl__clone_from_slice #t (x: t_Slice t) (y:t_Slice t) : t_Slice t = y
 
 val impl__split_at #t (s: t_Slice t) (mid: usize): Pure (t_Slice t * t_Slice t)
-    (requires (mid <=. length s))
-    (ensures (fun (x,y) -> length x == mid /\ length y == length s -. mid /\
-                        x == slice s (sz 0) mid /\ y == slice s mid (length s) /\
+    (requires (v mid <= length s))
+    (ensures (fun (x,y) -> length x == v mid /\ length y == length s - v mid /\
+                        x == slice s 0 (v mid) /\ y == slice s (v mid) (length s) /\
                         s == concat x y))
 
-let impl__is_empty (s: t_Slice 'a): bool = length s = sz 0
+let impl__is_empty (s: t_Slice 'a): bool = length s = 0
 
 let impl__contains (#t: eqtype) (s: t_Slice t) (v: t) =
   mem v s 
