proof-libs/fstar/rust_primitives/Rust_primitives.Hax.Folds.fsti
@@ -10,11 +10,11 @@ open FStar.Mul
 
 let nth_chunk_of #t
   (s: t_Slice t)
-  (s_chunk: t_Slice t {length s_chunk >. sz 0})
-  (chunk_nth: usize {chunk_nth <. (length s /! length s_chunk)})
+  (s_chunk: t_Slice t {length s_chunk > 0})
+  (chunk_nth: usize {v chunk_nth < (length s / length s_chunk)})
   : Type0
   =  
-  slice s (length s_chunk *! chunk_nth) (length s_chunk *! (chunk_nth +! sz 1))
+  slice s (length s_chunk * v chunk_nth) (length s_chunk * (v chunk_nth + 1))
   == s_chunk
 
 /// Fold function that is generated for `for` loops iterating on
@@ -23,13 +23,13 @@ val fold_enumerated_chunked_slice
   (#t: Type0) (#acc_t: Type0)
   (chunk_size: usize {v chunk_size > 0})
   (s: t_Slice t)
-  (inv: acc_t -> (i:usize{i <=. length s /! chunk_size}) -> Type0)
+  (inv: acc_t -> (i:usize{v i <= length s / v chunk_size}) -> Type0)
   (init: acc_t {inv init (sz 0)})
   (f: ( acc:acc_t
       -> item:(usize & t_Slice t) {
         let (i, s_chunk) = item in
-          i <. length s /! chunk_size
-        /\ length s_chunk == chunk_size
+          v i < length s / v chunk_size
+        /\ length s_chunk == v chunk_size
         /\ nth_chunk_of s s_chunk i
         /\ inv acc i
       }
@@ -38,7 +38,7 @@ val fold_enumerated_chunked_slice
       }
       )
   )
-  : result: acc_t {inv result (length s /! chunk_size)}
+  : result: acc_t {inv result (sz (length s / v chunk_size))}
 
 /// Fold function that is generated for `for` loops iterating on
 /// `s.chunks_exact(chunk_size)`-like iterators
@@ -50,7 +50,7 @@ val fold_chunked_slice
   (init: acc_t {inv init (sz 0)})
   (f: ( acc:acc_t
       -> item:(t_Slice t) {
-        length item == chunk_size /\
+        length item == v chunk_size /\
         inv acc (sz 0)
       }
       -> acc':acc_t {
@@ -66,18 +66,18 @@ val fold_chunked_slice
 val fold_enumerated_slice
   (#t: Type0) (#acc_t: Type0)
   (s: t_Slice t)
-  (inv: acc_t -> (i:usize{v i <= v (length s)}) -> Type0)
+  (inv: acc_t -> (i:usize{v i <= length s}) -> Type0)
   (init: acc_t {inv init (sz 0)})
-  (f: (acc:acc_t -> i:(usize & t) {v (fst i) < v (length s) /\ snd i == index s (fst i) /\ inv acc (fst i)}
-                 -> acc':acc_t    {v (fst i) < v (length s) /\ inv acc' (fst i)}))
-  : result: acc_t {inv result (length s)}
+  (f: (acc:acc_t -> i:(usize & t) {v (fst i) < length s /\ snd i == index s (v (fst i)) /\ inv acc (fst i)}
+                 -> acc':acc_t    {v (fst i) < length s /\ inv acc' (fst i)}))
+  : result: acc_t {inv result (sz (length s))}
 
 val fold_enumerated_slice_return
   (#t: Type0) (#acc_t: Type0) (#ret: Type0)
   (s: t_Slice t)
-  (inv: acc_t -> (i:usize{v i <= v (length s)}) -> Type0)
+  (inv: acc_t -> (i:usize{v i <= length s}) -> Type0)
   (init: acc_t {inv init (sz 0)})
-  (f: (acc:acc_t -> i:(usize & t) {v (fst i) < v (length s) /\ snd i == index s (fst i) (*/\ inv acc  (fst i)*)}
+  (f: (acc:acc_t -> i:(usize & t) {v (fst i) < length s /\ snd i == index s (v (fst i)) (*/\ inv acc  (fst i)*)}
                  -> Core.Ops.Control_flow.t_ControlFlow (Core.Ops.Control_flow.t_ControlFlow ret (unit & acc_t)) (acc':acc_t)    (*{v (fst i) < v (length s) /\ inv acc' (fst i)}*)))
   : result: Core.Ops.Control_flow.t_ControlFlow ret acc_t(* {inv result (length s)} *)
 
