proof-libs/fstar/rust_primitives/Rust_primitives.Hax.Monomorphized_update_at.fsti
@@ -10,55 +10,55 @@ open Core.Ops.Range
 let update_at_usize
   (#t: Type0)
   (s: t_Slice t)
-  (i: usize {i <. length s})
+  (i: usize {v i < length s})
   (x: t)
-  : t_Array t (length s)
-  = upd #t s i x
+  : t_Array t (sz (length s))
+  = upd #t s (v i) x
 
 val update_at_range #n
   (#t: Type0)
   (s: t_Slice t)
   (i: t_Range (int_t n))
   (x: t_Slice t)
-  : Pure (t_Array t (length s))
+  : Pure (t_Array t (sz (length s)))
     (requires (v i.f_start >= 0 /\ 
-               v i.f_start <= v (length s) /\
-               v i.f_end <= v (length s) /\
-               v (length x) == v i.f_end - v i.f_start))
+               v i.f_start <= length s /\
+               v i.f_end <= length s /\
+               length x == v i.f_end - v i.f_start))
     (ensures (fun res ->
-                slice res (sz 0) (sz (v i.f_start)) == slice s (sz 0) (sz (v i.f_start)) /\
-                slice res (sz (v i.f_start)) (sz (v i.f_end)) == x /\
-                slice res (sz (v i.f_end)) (length res) == slice s (sz (v i.f_end)) (length s)))
+                slice res 0 (v i.f_start) == slice s 0 (v i.f_start) /\
+                slice res (v i.f_start) (v i.f_end) == x /\
+                slice res (v i.f_end) (length res) == slice s (v i.f_end) (length s)))
 
 val update_at_range_to #n
   (#t: Type0)
   (s: t_Slice t)
   (i: t_RangeTo (int_t n))
   (x: t_Slice t)
-  : Pure (t_Array t (length s))
-    (requires (v i.f_end >= 0 /\ v i.f_end <= v (length s) /\
-               v (length x) == v i.f_end))
+  : Pure (t_Array t (sz (length s)))
+    (requires (v i.f_end >= 0 /\ v i.f_end <= length s /\
+               length x == v i.f_end))
     (ensures (fun res ->
-                slice res (sz 0) (sz (v i.f_end)) == x /\
-                slice res (sz (v i.f_end)) (length res) == slice s (sz (v i.f_end)) (length s)))
+                slice res 0 (v i.f_end) == x /\
+                slice res (v i.f_end) (length res) == slice s (v i.f_end) (length s)))
 
 val update_at_range_from #n
   (#t: Type0)
   (s: t_Slice t)
   (i: t_RangeFrom (int_t n))
   (x: t_Slice t)
-  : Pure (t_Array t (length s))
-    (requires ( v i.f_start >= 0 /\ v i.f_start <= v (length s) /\
-                v (length x) == v (length s) - v i.f_start))
+  : Pure (t_Array t (sz (length s)))
+    (requires ( v i.f_start >= 0 /\ v i.f_start <= length s /\
+                length x == length s - v i.f_start))
     (ensures (fun res ->
-                slice res (sz 0) (sz (v i.f_start)) == slice s (sz 0) (sz (v i.f_start)) /\
-                slice res (sz (v i.f_start)) (length res) == x))
+                slice res 0 (v i.f_start) == slice s 0 (v i.f_start) /\
+                slice res (v i.f_start) (length res) == x))
 
 val update_at_range_full
   (#t: Type0)
   (s: t_Slice t)
   (i: t_RangeFull)
   (x: t_Slice t)
-  : Pure (t_Array t (length s))
+  : Pure (t_Array t (sz (length s)))
     (requires (length x == length s))
     (ensures (fun res -> res == x))
