proof-libs/fstar/rust_primitives/Rust_primitives.Hax.fst
@@ -7,7 +7,7 @@ type t_Never = False
 let never_to_any #t: t_Never -> t = (fun _ -> match () with)
 
 let repeat #a (x: a) (len: usize): t_Array a len = 
-    createi len (fun i -> x)
+    createi (v len) (fun i -> x)
 
 open Core.Ops.Index
 class update_at_tc self idx = {
@@ -25,26 +25,26 @@ instance impl__index_refined t l n r: t_Index (t_Array t l) (x: int_t n {r x})
   = { f_Output = t;
       f_index_pre = (fun (s: t_Array t l) (i: int_t n {r i}) -> v i >= 0 && v i < v l);
       f_index_post = (fun _ _ _ -> true);
-      f_index = (fun s i -> index s (sz (v i)));
+      f_index = (fun s i -> index s (v i));
     }
 
 /// Similarly to `impl__index_refined`, we need to define a instance
 /// for refined `int_t n`.
 instance update_at_tc_array_refined t l n r: update_at_tc (t_Array t l) (x: int_t n {r x}) = {
   super_index = impl__index_refined t l n r;
-  update_at = (fun arr i x -> upd arr (sz (v i)) x);
+  update_at = (fun arr i x -> upd arr (v i) x);
 }
 
 instance impl__index t l n: t_Index (t_Array t l) (int_t n)
   = { f_Output = t;
       f_index_pre = (fun (s: t_Array t l) (i: int_t n) -> v i >= 0 && v i < v l);
       f_index_post = (fun _ _ _ -> true);
-      f_index = (fun s i -> index s (sz (v i)));
+      f_index = (fun s i -> index s (v i));
     }
 
 instance update_at_tc_array t l n: update_at_tc (t_Array t l) (int_t n) = {
   super_index = FStar.Tactics.Typeclasses.solve <: t_Index (t_Array t l) (int_t n);
-  update_at = (fun arr i x -> upd arr (sz (v i)) x);
+  update_at = (fun arr i x -> upd arr (v i) x);
 }
 
 let (.[]<-) #self #idx {| update_at_tc self idx |} (s: self) (i: idx {f_index_pre s i})
