proof-libs/fstar/core/Core.Ops.Index.IndexMut.fst
@@ -10,5 +10,5 @@ open Rust_primitives
 instance impl__index_mut t l n: t_IndexMut (t_Array t l) (int_t n)
   = { f_Input = t;
       in_range = (fun (s: t_Array t l) (i: int_t n) -> v i >= 0 && v i < v l);
-      f_index_mut = (fun s i x -> upd s (sz (v i)) x);
+      f_index_mut = (fun s i x -> upd s (v i) x);
     }
